small changes for linked lists + examples

state/LinkedListIFC.fst
@@ -13,29 +13,56 @@ noeq type linkedList (a: Type0) : Type0 =
     | Cons of a * ref (linkedList a)
 
 instance target_lang_linkedList (t1:Type) {| c1:target_lang t1 |} : target_lang (linkedList t1) = {
-  shallowly_witnessed_contains = (fun x ->
-    match x with
+  shallowly_contained = (fun l h ->
+    match l with
     | Nil -> True
-    | Cons (h, tl) -> c1.shallowly_witnessed_contains h /\ is_mm tl = false /\ witnessed (contains_pred tl)); 
-  shallowly_witnessed_is_low = (fun x ->
-    match x with
+    | Cons (x, xs) -> c1.shallowly_contained x h /\ is_mm xs = false /\ contains_pred xs h); 
+  shallowly_low = (fun l h ->
+    match l with
     | Nil -> True
-    | Cons (h, tl) -> c1.shallowly_witnessed_is_low h /\ witnessed (is_low_pred tl));
+    | Cons (x, xs) -> c1.shallowly_low x h /\ is_low_pred xs h);
+  shallowly_witness = (fun l ->
+    match l with 
+    | Nil -> (fun () -> ())
+    | Cons (x, xs) ->
+      let w = c1.shallowly_witness x in
+      gst_witness (contains_pred xs);
+      gst_witness (is_low_pred xs);
+      (fun () -> w ();
+       gst_recall (contains_pred xs);
+       gst_recall (is_low_pred xs))
+      )
 }
 
+// maybe change this to not use IST
 let head (a: Type0) (l:linkedList a) {| c1:target_lang a |} : IST (option a)
-  (requires (fun h -> shallowly_witnessed_contains l))
+  (requires (fun h -> shallowly_contained l h))
     (ensures fun _ _ _ -> True) = 
       match l with
       | Nil -> None
-      | Cons (h, tl) -> Some h
+      | Cons (x, xsref) -> Some x
 
 let tail (a: Type0) (l: linkedList a) {| c1:target_lang a |} : IST (linkedList a)
-    (requires (fun h -> shallowly_witnessed_contains l))
+    (requires (fun h -> shallowly_contained l h))
     (ensures fun _ _ _ -> True) = 
       match l with
       | Nil -> Nil
-      | Cons (h, tl) -> !tl
+      | Cons (x, xsref) -> !xsref
+
+let rec last (#a: Type0) (l:linkedList a) {| c1:target_lang a |} : IST (option a)
+  (requires (fun h -> shallowly_contained l h))
+  (ensures fun _ _ _ -> True) = 
+    let h0 = get() in
+    match l with 
+    | Nil -> None
+    | Cons (x, xsref) ->
+      let xs = !xsref in
+      match xs with
+      | Nil -> Some x
+      | Cons _ -> 
+        eliminate forall (a:Type) (c:target_lang a) (r':ref a). shallowly_contained r' h0 ==>
+          c.shallowly_contained (sel h0 r') h0 with (linkedList a) (solve) xsref;
+        last xs #c1
 
 let insert_front (a: Type0) (l: linkedList a) (v: a) {| c:target_lang a |}: ST (linkedList a)
     (requires (fun _ -> True))
@@ -59,18 +86,47 @@ let insert_front (a: Type0) (l: linkedList a) (v: a) {| c:target_lang a |}: ST (
 //         append a tl v #c
 
 let rec length (a: Type0) (l: linkedList a) {| c:target_lang a |} : IST nat 
-       (requires (fun h -> shallowly_witnessed_contains l /\ shallowly_witnessed_is_low l))
+       (requires (fun h -> shallowly_contained l h /\ shallowly_low l h))
        (ensures fun _ _ _ -> True) =
        let h0 = get() in
         match l with 
          | Nil -> 0
-         | Cons (h, tlref) -> 
-           let tl = !tlref in
-            eliminate forall (a:Type) (c:target_lang a) (r:ref a). witnessed (is_low_pred r) ==>
-              c.shallowly_witnessed_is_low (sel h0 r) with (linkedList a) (solve) tlref;
-            eliminate forall (a:Type) (c:target_lang a) (r:ref a). witnessed (contains_pred r) ==>
-              c.shallowly_witnessed_contains (sel h0 r) with (linkedList a) (solve) tlref;
-            1 + length a tl #c
+         | Cons (x, xsref) -> 
+           let xs = !xsref in
+            eliminate forall (a:Type) (c:target_lang a) (r:ref a). shallowly_low r h0 ==>
+              c.shallowly_low (sel h0 r) h0 with (linkedList a) (solve) xsref;
+            eliminate forall (a:Type) (c:target_lang a) (r:ref a). shallowly_contained r h0 ==>
+              c.shallowly_contained (sel h0 r) h0 with (linkedList a) (solve) xsref;
+            1 + length a xs #c
+
+// cycles??
+let rec ll_eq (#a: Type0) (fuel: nat) (l1: linkedList a) (l2: linkedList a) (h: lheap) : Type0 =
+  if fuel = 0 then True
+  else
+    match (l1, l2) with
+    | (Nil, Nil) -> true
+    | Nil, _ -> false
+    | _, Nil -> false
+    | (Cons (x, xsref), Cons (y, ysref)) ->
+      let xs = sel h xsref in
+      let ys = sel h ysref in  
+      x == y /\ ll_eq (fuel - 1) xs ys h
+
+let rec ll_constant (#a: Type0) (fuel: nat) (l: linkedList a) (h1 h2: lheap) : Type0 =
+  if fuel = 0 then True
+  else
+    match l with
+    | Nil -> True
+    | Cons (_, xsref) -> begin
+      let xs1 = sel h1 xsref in
+      let xs2 = sel h2 xsref in
+      match (xs1, xs2) with
+      | (Nil, Nil) -> True
+      | Nil, _ -> False
+      | _, Nil -> False
+      | (Cons (x, xsref), Cons (y, ysref)) ->
+        x == y /\ xsref == ysref /\ ll_constant (fuel - 1) xs1 h1 h2
+    end
 
 // examples
 
@@ -90,75 +146,161 @@ let cycle_length3 () : ST (linkedList nat) (requires fun _ -> True) (ensures fun
     let x = alloc Nil in 
     let y = alloc (Cons (7, x)) in
     let z = alloc (Cons (5, y)) in 
-    gst_witness (contains_pred x);
+    // gst_witness (contains_pred x);
     write x (Cons(2, z));
     Cons (2, z)
 
 
 // TODO: clean up
 let rec deep_declassify (l: linkedList int) : ST unit 
-  (requires fun h -> shallowly_witnessed_contains l /\ inv_contains_points_to_contains h)
-  (ensures fun h0 x h1 -> (inv_contains_points_to_contains h1) /\
-                           modifies Set.empty h0 h1 /\
-                           shallowly_witnessed_is_low l /\
-                           (forall (a:Type) (c:target_lang a) (r:ref a). 
-                           (h0 `contains` r /\ label_of r h0 <> Low /\ label_of r h1 == Low) ==> c.shallowly_witnessed_is_low (sel h1 r) )
-                           ) =
+  (requires fun h -> shallowly_contained l h /\ inv_contains_points_to_contains h)
+  (ensures fun h0 x h1 ->
+    inv_contains_points_to_contains h1 /\
+    modifies Set.empty h0 h1 /\
+    shallowly_low l h1 /\
+    (forall (a:Type) (c:target_lang a) (r:ref a). 
+    (shallowly_contained r h0 /\ ~(shallowly_low r h0) /\ shallowly_low r h1) ==> c.shallowly_low (sel h1 r) h1)
+    ) =
   let h0 = get() in
   match l with 
   | Nil -> ()
   | Cons (h, tlref) ->
-    let tl = !tlref in 
-      declassify tlref Low;
-      gst_witness (is_low_pred tlref);
-      eliminate forall (a:Type) (c:target_lang a) (r:ref a). witnessed (contains_pred r) ==>
-        c.shallowly_witnessed_contains (sel h0 r) with (linkedList int) (solve) tlref;
+      let tl = !tlref in 
+      declassify_low' tlref;
+      // gst_witness (is_low_pred tlref);
+      eliminate forall (a:Type) (c:target_lang a) (r:ref a). shallowly_contained r h0 ==>
+        c.shallowly_contained (sel h0 r) h0 with (linkedList int) (solve) tlref;
       let h1 = get () in
+      // admit();
       deep_declassify tl;
+      // admit();
       let h2 = get () in
-      assert ((forall (a:Type) (c:target_lang a) (r:ref a). h0 `contains` r <==> h1 `contains` r));
-      assert ((forall (a:Type) (c:target_lang a) (r:ref a). 
-                (h1 `contains` r /\ label_of r h1 <> Low /\ label_of r h2 == Low) ==> 
-                  c.shallowly_witnessed_is_low (sel h2 r) ));
+      // assert ((forall (a:Type) (c:target_lang a) (r:ref a). h0 `contains` r <==> h1 `contains` r));
+      // assert ((forall (a:Type) (c:target_lang a) (r:ref a). 
+      //           (h1 `contains` r /\ label_of r h1 <> Low /\ label_of r h2 == Low) ==> 
+      //             c.shallowly_low (sel h2 r) h2));
 
 
-      assert (modifies_classification (only tlref) h0 h1);
-      assert (modifies Set.empty h0 h2);
-      assert (sel h0 tlref == sel h2 tlref);
-      assert (shallowly_witnessed_is_low (sel h2 tlref));
-      assert ((label_of tlref h0 <> Low /\ label_of tlref h2 == Low) ==> 
-                shallowly_witnessed_is_low (sel h2 tlref) );   
+      // assert (modifies_classification (only tlref) h0 h1);
+      // assert (modifies Set.empty h0 h2);
+      // assert (sel h0 tlref == sel h2 tlref);
+      // assert (shallowly_low (sel h2 tlref) h2);
+      // assert ((label_of tlref h0 <> Low /\ label_of tlref h2 == Low) ==> 
+      //           shallowly_low (sel h2 tlref) h2);   
     
       introduce forall (a:Type) (c:target_lang a) (r:ref a). 
-               (h0 `contains` r /\ label_of r h0 <> Low /\ label_of r h2 == Low) ==> 
-                c.shallowly_witnessed_is_low (sel h2 r)
+               (shallowly_contained r h0 /\ ~(shallowly_low r h0) /\ shallowly_low r h2) ==> 
+                c.shallowly_low (sel h2 r) h2
       with begin
-        introduce (h0 `contains` r /\ label_of r h0 <> Low /\ label_of r h2 == Low) ==> 
-                c.shallowly_witnessed_is_low (sel h2 r)
+        introduce (shallowly_contained r h0 /\ ~(shallowly_low r h0) /\ shallowly_low r h2) ==> 
+                c.shallowly_low (sel h2 r) h2
         with _. begin
-          introduce label_of r h1 <> Low ==> c.shallowly_witnessed_is_low (sel h2 r) with _. ();
-          introduce label_of r h1 == Low ==> c.shallowly_witnessed_is_low (sel h2 r) with _. begin
+          introduce ~(shallowly_low r h1) ==> c.shallowly_low (sel h2 r) h2 with _. ();
+          introduce shallowly_low r h1 ==> c.shallowly_low (sel h2 r) h2 with _. begin
             assert (addr_of r = addr_of tlref);
-            assume (is_mm r == is_mm tlref);
             lemma_sel_same_addr' h2 r tlref;
-            assert (shallowly_witnessed_is_low (sel h2 tlref));
+            assert (shallowly_low (sel h2 tlref) h2);
             assert (sel h2 tlref == sel h2 r);
             // let r : ref (linkedList int) = r in
             let c : target_lang (linkedList int) = c in
-            assert ((target_lang_linkedList int).shallowly_witnessed_is_low (sel h2 tlref));
+            assert ((target_lang_linkedList int).shallowly_low (sel h2 tlref) h2);
             assume ((forall (a:Type) (c:target_lang a) (c':target_lang a) (v:a) . 
-              c.shallowly_witnessed_is_low v ==> c'.shallowly_witnessed_is_low v));
-            assert (c.shallowly_witnessed_is_low (sel h2 tlref));
-            assert (c.shallowly_witnessed_is_low (sel h2 r));
+              c.shallowly_low v h2 ==> c'.shallowly_low v h2));
+            assert (c.shallowly_low (sel h2 tlref) h2);
+            assert (c.shallowly_low (sel h2 r) h2);
             ()
           end
         end 
       end;
-      assert ((forall (a:Type) (c:target_lang a) (r:ref a). 
-          (h0 `contains` r /\ label_of r h0 <> Low /\ label_of r h2 == Low) ==> 
-          c.shallowly_witnessed_is_low (sel h2 r) ));
       ()
 
-  // let test (l: linkedList int) : IST unit (ensures fun _ -> True) (requires fun _ _ _ -> True) =
-  //   deep_declassify l;
-  //   ()
+  // Tests
+
+
+// review this later
+let test_declassify (l: linkedList int) : IST unit (ensures fun h -> shallowly_contained l h) (requires fun _ _ _ -> True) =
+  // deep_declassify l;
+  // let h2 = get() in
+  // assume ((forall (a:Type) (c:target_lang a) (c':target_lang a) (v:a) . 
+  //            c.shallowly_low v h2 ==> c'.shallowly_low v h2));
+  ()
+
+val progr_linked_list_unchanged: 
+  rp: ref (linkedList int) -> 
+  rs: ref int ->
+  ctx:(elab_typ (TArr TUnit TUnit)) ->
+  IST unit 
+    (requires (fun h0 -> 
+      shallowly_contained rp h0 /\
+      label_of rp h0 == High /\
+      shallowly_low rs h0))
+    (ensures (fun h0 _ h1 ->
+      sel h0 rp == sel h1 rp))
+         
+let progr_secret_unchanged_test rp rs ctx = 
+  let x = alloc Nil in 
+  let y = alloc (Cons (31, x)) in
+  let secret_ll = Cons(23, y) in
+  ctx ();
+  // assert (head int secret_ll == 31); // how to cast type?
+  // assert (head int (tail int secret_ll) == 23);
+  ()
+
+// val ctx_HO :
+//   elab_typ (TArr (TArr TUnit (TRef TNat)) TUnit)
+// let ctx_HO f =
+//   let h0 = get () in
+//   let x:ref int = f () in
+//   let y = alloc Nil in
+//   let z = Cons(!x, y) in
+//   let t = insert_front int z 13 in
+//   let h2 = get () in
+//   assert (modifies_only_label Low h0 h2);
+//   ()
+
+// test with program getting callback?
+
+
+// how to check all labels of a list are High (esp. for cycles?)?
+// val progr_sep:
+//   rp: linkedList int -> 
+//   ctx:(elab_typ (TArr (TRef TNat) TUnit)) ->
+//   IST unit
+//     (requires (fun h0 -> 
+//       shallowly_contained rp h0 /\
+//       // label_of (last rp) h0 == High)
+//     ))
+//     (ensures (fun h0 _ h1 -> True))
+// let progr_sep rp f =
+//   deep_declassify rp;
+//   let h1 = get () in
+//   assume (inv_low_points_to_low h1);
+//   let r = f rp in  
+//   r
+
+// val lemma_list_unchanged_when_high (#a: Type0) (rp: linkedList a) (h0 h1: lheap): Lemma {
+
+// }
+
+
+let rec deep_high_ll (#a: Type0) (fuel: nat) (l: linkedList a) (h: lheap): Type0 =
+  if fuel = 0 then True
+  else
+    match l with
+    | Nil -> True
+    | Cons (x, xsref) -> 
+      label_of xsref h == High /\ deep_high_ll (fuel - 1) (sel h xsref) h
+
+val progr_ll_unchanged':
+  rp: linkedList int -> 
+  ctx:(elab_typ (TArr TUnit TUnit)) ->
+  IST unit
+    (requires (fun h0 -> 
+      (forall gas . deep_high_ll gas rp h0) /\
+      shallowly_contained rp h0
+    ))
+    (ensures (fun h0 _ h1 ->  forall gas . ll_constant gas rp h0 h1))
+let progr_ll_unchanged' rp f =
+  let h1 = get () in
+  f ();
+  ()
